Finally derived the recursion equations for decode_list.

src/Boolify/src/CoderScript.sml
@@ -56,7 +56,7 @@ end;
 val wf_pdecoder_def = Define
   `wf_pdecoder p (d : bool list -> ('a # bool list) option) =
    !x.
-     if x IN p then (?a. !b c. (d b = SOME (x, c)) = (b = APPEND a c))
+     if p x then (?a. !b c. (d b = SOME (x, c)) = (b = APPEND a c))
      else !a b. ~(d a = SOME (x, b))`;
 
 (*---------------------------------------------------------------------------
@@ -66,8 +66,8 @@ val wf_pdecoder_def = Define
 
 val enc2dec_def = Define
   `enc2dec p e (l : bool list) =
-   if ?x t. (x : 'a) IN p /\ (l = APPEND (e x) t)
-   then SOME (@(x, t). x IN p /\ (l = APPEND (e x) t))
+   if ?x t. p (x : 'a) /\ (l = APPEND (e x) t)
+   then SOME (@(x, t). p x /\ (l = APPEND (e x) t))
    else NONE`;
 
 val dec2enc_def = Define
@@ -80,8 +80,7 @@ val dec2enc_def = Define
 
 val enc2dec_none = store_thm
   ("enc2dec_none",
-   ``!p e l.
-       (enc2dec p e l = NONE) = (!x t. x IN p ==> ~(l = APPEND (e x) t))``,
+   ``!p e l. (enc2dec p e l = NONE) = (!x t. p x ==> ~(l = APPEND (e x) t))``,
    RW_TAC std_ss [enc2dec_def] ++
    PROVE_TAC []);
 
@@ -89,7 +88,7 @@ val enc2dec_some = store_thm
   ("enc2dec_some",
    ``!p e l x t.
        wf_pencoder p e ==>
-       ((enc2dec p e l = SOME (x, t)) = x IN p /\ (l = APPEND (e x) t))``,
+       ((enc2dec p e l = SOME (x, t)) = p x /\ (l = APPEND (e x) t))``,
    REVERSE (RW_TAC std_ss [enc2dec_def]) >> PROVE_TAC [] ++
    ONCE_REWRITE_TAC [GSYM (ONCE_DEPTH_CONV ETA_CONV ``@p. q p``)] ++
    SELECT_TAC ++
@@ -107,27 +106,27 @@ val enc2dec_some = store_thm
    SIMP_TAC std_ss [] ++
    REPEAT (DISCH_THEN STRIP_ASSUME_TAC) ++
    Suff `q = x` >> PROVE_TAC [APPEND_11] ++
-   FULL_SIMP_TAC std_ss [wf_pencoder_def, RES_FORALL_DEF] ++
+   FULL_SIMP_TAC std_ss [wf_pencoder_def] ++
    PROVE_TAC [IS_PREFIX_APPEND1, IS_PREFIX_APPEND2, IS_PREFIX_REFL]);
 
 val wf_enc2dec = store_thm
   ("wf_enc2dec",
    ``!p e. wf_pencoder p e ==> wf_pdecoder p (enc2dec p e)``,
-   RW_TAC std_ss [wf_pdecoder_def, enc2dec_some, RES_FORALL_DEF] ++
+   RW_TAC std_ss [wf_pdecoder_def, enc2dec_some] ++
    PROVE_TAC [APPEND_NIL]);
 
 val dec2enc_some = store_thm
   ("dec2enc_some",
    ``!p d x l.
        wf_pdecoder p d ==>
-       ((dec2enc d x = l) /\ x IN p = (d l = SOME (x, [])))``,
+       ((dec2enc d x = l) /\ p x = (d l = SOME (x, [])))``,
    RW_TAC std_ss [dec2enc_def] ++
    SELECT_TAC ++
    RW_TAC std_ss [] ++
    EQ_TAC >>
    (RW_TAC std_ss [] ++
     Q.PAT_ASSUM `X ==> Y` MATCH_MP_TAC ++
-    FULL_SIMP_TAC std_ss [wf_pdecoder_def, RES_FORALL_DEF] ++
+    FULL_SIMP_TAC std_ss [wf_pdecoder_def] ++
     PROVE_TAC [APPEND_NIL]) ++
    POP_ASSUM MP_TAC ++
    MATCH_MP_TAC
@@ -136,7 +135,7 @@ val dec2enc_some = store_thm
    POP_ASSUM MP_TAC ++
    SIMP_TAC std_ss [wf_pdecoder_def] ++
    DISCH_THEN (MP_TAC o Q.SPEC `x`) ++
-   REVERSE (Cases_on `x IN p`) >> PROVE_TAC [] ++
+   REVERSE (Cases_on `p x`) >> PROVE_TAC [] ++
    ASM_REWRITE_TAC [] ++
    DISCH_THEN (CHOOSE_THEN MP_TAC) ++
    RW_TAC std_ss []);
@@ -144,13 +143,13 @@ val dec2enc_some = store_thm
 val decode_dec2enc = store_thm
   ("decode_dec2enc",
    ``!p d x.
-       wf_pdecoder p d /\ x IN p ==> (d (dec2enc d x) = SOME (x, []))``,
+       wf_pdecoder p d /\ p x ==> (d (dec2enc d x) = SOME (x, []))``,
    PROVE_TAC [dec2enc_some]);
 
 val decode_dec2enc_append = store_thm
   ("decode_dec2enc_append",
    ``!p d x t.
-       wf_pdecoder p d /\ x IN p ==>
+       wf_pdecoder p d /\ p x ==>
        (d (APPEND (dec2enc d x) t) = SOME (x, t))``,
    RW_TAC std_ss [] ++
    MP_TAC (Q.SPECL [`p`, `d`, `x`] decode_dec2enc) ++
@@ -165,25 +164,25 @@ val decode_dec2enc_append = store_thm
 val wf_dec2enc = store_thm
   ("wf_dec2enc",
    ``!p d. wf_pdecoder p d ==> wf_pencoder p (dec2enc d)``,
-   RW_TAC std_ss [wf_pencoder_def, RES_FORALL_DEF] ++
+   RW_TAC std_ss [wf_pencoder_def] ++
    MP_TAC (Q.SPECL [`p`, `d`] wf_pdecoder_def) ++
    ASM_REWRITE_TAC [] ++
-   DISCH_THEN (fn th => MP_TAC (Q.SPEC `x` th) THEN MP_TAC (Q.SPEC `x'` th)) ++
+   DISCH_THEN (fn th => MP_TAC (Q.SPEC `x` th) THEN MP_TAC (Q.SPEC `y` th)) ++
    RW_TAC std_ss [] ++
    MP_TAC (Q.SPECL [`p`, `d`, `x`] decode_dec2enc) ++
-   MP_TAC (Q.SPECL [`p`, `d`, `x'`] decode_dec2enc) ++
+   MP_TAC (Q.SPECL [`p`, `d`, `y`] decode_dec2enc) ++
    RW_TAC std_ss [APPEND_NIL] ++
    POP_ASSUM MP_TAC ++
    POP_ASSUM MP_TAC ++
    POP_ASSUM (CHOOSE_THEN MP_TAC o REWRITE_RULE [IS_PREFIX_APPEND]) ++
    RW_TAC std_ss [GSYM APPEND_ASSOC] ++
-   POP_ASSUM (MP_TAC o Q.SPECL [`APPEND (dec2enc d x') l`, `[]`]) ++
-   POP_ASSUM (MP_TAC o Q.SPECL [`APPEND (dec2enc d x') l`, `l`]) ++
+   POP_ASSUM (MP_TAC o Q.SPECL [`APPEND (dec2enc d y) l`, `[]`]) ++
+   POP_ASSUM (MP_TAC o Q.SPECL [`APPEND (dec2enc d y) l`, `l`]) ++
    RW_TAC std_ss [APPEND_NIL]);
 
 val dec2enc_enc2dec = store_thm
   ("dec2enc_enc2dec",
-   ``!p e x. wf_pencoder p e /\ x IN p ==> (dec2enc (enc2dec p e) x = e x)``,
+   ``!p e x. wf_pencoder p e /\ p x ==> (dec2enc (enc2dec p e) x = e x)``,
    RW_TAC std_ss [] ++
    MP_TAC (Q.SPECL [`p`, `e`] wf_enc2dec) ++
    RW_TAC std_ss [dec2enc_some] ++
@@ -219,7 +218,7 @@ val enc2dec_dec2enc = store_thm
 
 val decode_encode = store_thm
   ("decode_encode",
-   ``!p e x. wf_pencoder p e /\ x IN p ==> (decode (enc2dec p e) (e x) = x)``,
+   ``!p e x. wf_pencoder p e /\ p x ==> (decode (enc2dec p e) (e x) = x)``,
    RW_TAC std_ss [] ++
    Cases_on `enc2dec p e (e x)` >>
    (POP_ASSUM MP_TAC ++
@@ -230,42 +229,27 @@ val decode_encode = store_thm
    SIMP_TAC std_ss [decode_def, o_THM] ++
    RW_TAC std_ss [enc2dec_some] ++
    MP_TAC (Q.SPECL [`p`, `e`] wf_pencoder_def) ++
-   RW_TAC std_ss [RES_FORALL_DEF] ++
+   RW_TAC std_ss [] ++
    Suff `IS_PREFIX (e x) (e q)` >> PROVE_TAC [] ++
    PROVE_TAC [IS_PREFIX_APPEND]);
 
 val encode_decode = store_thm
   ("encode_decode",
-   ``!p e l.
-       wf_pencoder p e /\ l IN domain (enc2dec p e) ==>
-       (e (decode (enc2dec p e) l) = l)``,
-   RW_TAC std_ss [domain_def, decode_def, o_THM] ++
+   ``!p e. !l :: domain (enc2dec p e).
+       wf_pencoder p e ==> (e (decode (enc2dec p e) l) = l)``,
+   RW_TAC std_ss [RES_FORALL_DEF, domain_def, decode_def, o_THM] ++
    RW_TAC std_ss [] ++
-   POP_ASSUM MP_TAC ++
+   Q.PAT_ASSUM `X = Y` MP_TAC ++
    RW_TAC std_ss [enc2dec_some, APPEND_NIL]);
-
-(* obsolete?
-val enc2dec_11 = store_thm
-  ("enc2dec_11",
-  ``!e f.
-       wf_encoder e /\ wf_encoder f /\ (enc2dec e = enc2dec f) ==> (e = f)``,
-   RW_TAC std_ss [] ++
-   MATCH_MP_TAC EQ_EXT ++
-   RW_TAC std_ss [] ++
-   MP_TAC (Q.SPECL [`e`, `e x`, `x`, `[]`] enc2dec_some) ++
-   RW_TAC std_ss [APPEND_NIL] ++
-   MP_TAC (Q.SPECL [`f`, `e x`, `x`, `[]`] enc2dec_some) ++
-   RW_TAC std_ss [APPEND_NIL]);
-*)
 
 (*---------------------------------------------------------------------------
      We define decoders in terms of encoders.
  ---------------------------------------------------------------------------*)
 
-val decode_bool_def = Define `decode_bool = enc2dec tot encode_bool`;
+val decode_bool_def = Define `decode_bool = enc2dec total encode_bool`;
 
 val decode_list_def = Define
-  `decode_list d = enc2dec tot (encode_list (dec2enc d))`;
+  `decode_list p d = enc2dec p (encode_list (dec2enc d))`;
 
 (*---------------------------------------------------------------------------
      decoders are well-formed and satisfy natural recursion equations.
@@ -273,21 +257,20 @@ val decode_list_def = Define
 
 val wf_decode_bool = store_thm
   ("wf_decode_bool",
-   ``wf_pdecoder tot decode_bool``,
+   ``wf_pdecoder total decode_bool``,
    RW_TAC std_ss [decode_bool_def, wf_enc2dec, wf_encoder, wf_encode_bool]);
 
 val decode_encode_bool = store_thm
   ("decode_encode_bool",
    ``!x. decode decode_bool (encode_bool x) = x``,
    RW_TAC std_ss
-   [decode_encode, decode_bool_def, wf_encoder, wf_encode_bool, tot_def]);
+   [decode_encode, decode_bool_def, wf_encoder, wf_encode_bool, total_def]);
 
 val encode_decode_bool = store_thm
   ("encode_decode_bool",
    ``!l :: domain decode_bool. encode_bool (decode decode_bool l) = l``,
-   RW_TAC std_ss
-   [RES_FORALL_DEF, encode_decode, decode_bool_def, wf_encoder,
-    wf_encode_bool, tot_def]);
+   MP_TAC (Q.ISPECL [`total : bool -> bool`, `encode_bool`] encode_decode) ++
+   RW_TAC std_ss [decode_bool_def, wf_encoder, wf_encode_bool, total_def]);
 
 val decode_bool = store_thm
   ("decode_bool",
@@ -295,29 +278,114 @@ val decode_bool = store_thm
    REPEAT CASE_TAC ++
    RW_TAC std_ss
    [decode_bool_def, enc2dec_none, enc2dec_some, encode_bool_def,
-    APPEND, wf_encode_bool, wf_encoder, tot_def]);
+    APPEND, wf_encode_bool, wf_encoder, total_def]);
 
-(* in progress
+val wf_decode_list = store_thm
+  ("wf_decode_list",
+   ``!p d.
+       wf_pdecoder p d ==> wf_pdecoder (EVERY p) (decode_list (EVERY p) d)``,
+   RW_TAC std_ss [decode_list_def] ++
+   PROVE_TAC [wf_dec2enc, wf_enc2dec, wf_pencode_list]);
+
+(* in progress ***
+val decode_encode_list = store_thm
+  ("decode_encode_list",
+   ``!p e x.
+       wf_pencoder p e /\ EVERY p x ==>
+       (decode (decode_list (EVERY p) (enc2dec p e)) (encode_list e x) = x)``,
+   RW_TAC std_ss [decode_encode, wf_pencode_list]
+decode_bool_def, wf_encoder, wf_encode_bool, total_def]);
+
+val encode_decode_bool = store_thm
+  ("encode_decode_bool",
+   ``!l :: domain decode_bool. encode_bool (decode decode_bool l) = l``,
+   MP_TAC (Q.ISPECL [`total : bool -> bool`, `encode_bool`] encode_decode) ++
+   RW_TAC std_ss [decode_bool_def, wf_encoder, wf_encode_bool, total_def]);
+*)
+
 val decode_list = store_thm
   ("decode_list",
-   ``(decode_list d l =
+   ``wf_pdecoder p d ==>
+     (decode_list (EVERY p) d l =
       case l of [] -> NONE
       || (T :: t) ->
          (case d t of NONE -> NONE
           || SOME (x, t') ->
-             (case decode_list d t' of NONE -> NONE
+             (case decode_list (EVERY p) d t' of NONE -> NONE
               || SOME (xs, t'') -> SOME (x :: xs, t'')))
       || (F :: t) -> SOME ([], t))``,
    (REPEAT CASE_TAC ++
-    RW_TAC std_ss [decode_list_def, enc2dec_none, tot_def]) <<
+    RW_TAC std_ss [decode_list_def, enc2dec_none]) <<
    [Cases_on `x` ++
     RW_TAC std_ss [encode_list_def, APPEND],
     Cases_on `x` ++
-    RW_TAC std_ss [encode_list_def, APPEND, GSYM APPEND_ASSOC] ++
+    POP_ASSUM MP_TAC ++
+    RW_TAC std_ss [encode_list_def, APPEND, GSYM APPEND_ASSOC, EVERY_DEF] ++
+    POP_ASSUM (K ALL_TAC) ++
+    Q.SPEC_TAC (`APPEND (encode_list (dec2enc d) t'') t'`, `l`) ++
+    REPEAT STRIP_TAC ++
+    RW_TAC std_ss [] ++
+    MP_TAC (Q.SPECL [`p`, `d`] wf_pdecoder_def) ++
+    RW_TAC std_ss [] ++
+    Q.EXISTS_TAC `h` ++
+    RW_TAC std_ss [] ++
+    PROVE_TAC [decode_dec2enc_append, NOT_SOME_NONE],
+    Cases_on `x` ++
+    POP_ASSUM MP_TAC ++
+    RW_TAC std_ss [encode_list_def, APPEND, GSYM APPEND_ASSOC, EVERY_DEF] ++
     STRIP_TAC ++
-    RW_TAC std_ss []
-    
-); 
-*)
+    RW_TAC std_ss [] ++
+    Q.PAT_ASSUM `X = SOME Y` MP_TAC ++
+    MP_TAC (Q.SPECL [`p`, `d`, `h`] decode_dec2enc_append) ++
+    ASM_SIMP_TAC std_ss [] ++
+    DISCH_THEN (K ALL_TAC) ++
+    PURE_REWRITE_TAC [GSYM DE_MORGAN_THM] ++
+    STRIP_TAC ++
+    RW_TAC std_ss [] ++
+    Q.PAT_ASSUM `X = Y` MP_TAC ++
+    RW_TAC std_ss [decode_list_def, enc2dec_none] ++
+    PROVE_TAC [],
+    Know `wf_pdecoder (EVERY p) (decode_list (EVERY p) d)` >>
+    PROVE_TAC [wf_decode_list] ++
+    STRIP_TAC ++
+    Know `wf_pencoder p (dec2enc d)` >> PROVE_TAC [wf_dec2enc] ++
+    STRIP_TAC ++
+    Know `wf_pencoder (EVERY p) (encode_list (dec2enc d))` >>
+    PROVE_TAC [wf_pencode_list] ++
+    STRIP_TAC ++
+    ASM_SIMP_TAC std_ss [enc2dec_some, encode_list_def, APPEND] ++
+    MATCH_MP_TAC (PROVE [] ``x /\ (x ==> y) ==> x /\ y``) ++
+    CONJ_TAC >> PROVE_TAC [EVERY_DEF, wf_pdecoder_def, wf_decode_list] ++
+    RW_TAC std_ss [EVERY_DEF] ++
+    MP_TAC (Q.SPECL [`p`, `d`] wf_pdecoder_def) ++
+    ASM_SIMP_TAC std_ss [] ++
+    DISCH_THEN (MP_TAC o Q.SPEC `q`) ++
+    RW_TAC std_ss [] ++
+    RES_TAC ++
+    RW_TAC std_ss [GSYM APPEND_ASSOC] ++
+    Know `dec2enc d q = a` >> PROVE_TAC [APPEND_NIL, dec2enc_some] ++
+    RW_TAC std_ss [APPEND_11] ++
+    Q.PAT_ASSUM `!x. P x` (K ALL_TAC) ++
+    MP_TAC
+    (Q.ISPECL [`EVERY (p : 'a -> bool)`, `decode_list (EVERY p) d`]
+     wf_pdecoder_def) ++
+    ASM_SIMP_TAC std_ss [] ++
+    DISCH_THEN (MP_TAC o Q.SPEC `q'`) ++
+    RW_TAC std_ss [] ++
+    RES_TAC ++
+    RW_TAC std_ss [] ++
+    Q.PAT_ASSUM `!x. P x` (K ALL_TAC) ++
+    Q.PAT_ASSUM `X = Y` MP_TAC ++
+    ASM_SIMP_TAC std_ss [decode_list_def, enc2dec_some],
+    Know `wf_pdecoder (EVERY p) (decode_list (EVERY p) d)` >>
+    PROVE_TAC [wf_decode_list] ++
+    STRIP_TAC ++
+    Know `wf_pencoder p (dec2enc d)` >> PROVE_TAC [wf_dec2enc] ++
+    STRIP_TAC ++
+    Know `wf_pencoder (EVERY p) (encode_list (dec2enc d))` >>
+    PROVE_TAC [wf_pencode_list] ++
+    STRIP_TAC ++
+    ASM_SIMP_TAC std_ss [enc2dec_some, encode_list_def, APPEND, EVERY_DEF]]);
 
 val _ = export_theory ();
+
